coq/map.v
@@ -12,7 +12,7 @@ Definition ___builtin_clz : ident := 22%positive.
 Definition ___compcert_va_int64 : ident := 17%positive.
 Definition ___builtin_memcpy_aligned : ident := 8%positive.
 Definition ___builtin_subl : ident := 5%positive.
-Definition _main : ident := 50%positive.
+Definition _size_rec : ident := 50%positive.
 Definition _find_key : ident := 43%positive.
 Definition ___builtin_va_start : ident := 12%positive.
 Definition _value : ident := 47%positive.
@@ -38,6 +38,7 @@ Definition _key : ident := 42%positive.
 Definition ___builtin_bswap16 : ident := 21%positive.
 Definition ___compcert_va_float64 : ident := 18%positive.
 Definition ___builtin_annot : ident := 9%positive.
+Definition _main : ident := 52%positive.
 Definition _val : ident := 45%positive.
 Definition _keys : ident := 41%positive.
 Definition ___builtin_va_arg : ident := 13%positive.
@@ -50,16 +51,17 @@ Definition ___builtin_fnmadd : ident := 29%positive.
 Definition _busybits : ident := 35%positive.
 Definition ___builtin_fnmsub : ident := 30%positive.
 Definition ___builtin_ctz : ident := 23%positive.
+Definition _size : ident := 51%positive.
 Definition _put : ident := 48%positive.
 Definition ___builtin_bswap32 : ident := 20%positive.
-Definition _index'1 : ident := 53%positive.
-Definition _start'1 : ident := 57%positive.
-Definition _start'2 : ident := 59%positive.
-Definition _index'3 : ident := 58%positive.
-Definition _index'2 : ident := 56%positive.
-Definition _index'4 : ident := 60%positive.
-Definition _start' : ident := 55%positive.
-Definition _index' : ident := 51%positive.
+Definition _index'4 : ident := 62%positive.
+Definition _index' : ident := 53%positive.
+Definition _start' : ident := 57%positive.
+Definition _start'2 : ident := 61%positive.
+Definition _start'1 : ident := 59%positive.
+Definition _index'2 : ident := 58%positive.
+Definition _index'3 : ident := 60%positive.
+Definition _index'1 : ident := 55%positive.
 
 
 Definition f_loop := {|
@@ -83,7 +85,7 @@ Definition f_find_empty := {|
   fn_params := ((_busybits, (tptr tint)) :: (_start, tint) :: (_i, tint) ::
                 nil);
   fn_vars := nil;
-  fn_temps := ((_index, tint) :: (_bb, tint) :: (52%positive, tint) ::
+  fn_temps := ((_index, tint) :: (_bb, tint) :: (54%positive, tint) ::
                (_index', tint) :: nil);
   fn_body :=
 (Ssequence
@@ -110,7 +112,7 @@ Definition f_find_empty := {|
           (Sreturn (Some (Eunop Oneg (Econst_int (Int.repr 1) tint) tint)))
           Sskip)
         (Ssequence
-          (Scall (Some 52%positive)
+          (Scall (Some 54%positive)
             (Evar _find_empty (Tfunction
                                 (Tcons (tptr tint)
                                   (Tcons tint (Tcons tint Tnil))) tint
@@ -118,7 +120,7 @@ Definition f_find_empty := {|
             ((Etempvar _busybits (tptr tint)) :: (Etempvar _start tint) ::
              (Ebinop Osub (Etempvar _i tint) (Econst_int (Int.repr 1) tint)
                tint) :: nil))
-          (Sreturn (Some (Etempvar 52%positive tint))))))))
+          (Sreturn (Some (Etempvar 54%positive tint))))))))
 |}.
 
 Definition f_find_key := {|
@@ -128,7 +130,7 @@ Definition f_find_key := {|
                 (_start, tint) :: (_key, tint) :: (_i, tint) :: nil);
   fn_vars := nil;
   fn_temps := ((_index, tint) :: (_bb, tint) :: (_k, tint) ::
-               (54%positive, tint) :: (_index'1, tint) :: nil);
+               (56%positive, tint) :: (_index'1, tint) :: nil);
   fn_body :=
 (Ssequence
   (Ssequence
@@ -162,7 +164,7 @@ Definition f_find_key := {|
             (Sreturn (Some (Eunop Oneg (Econst_int (Int.repr 1) tint) tint)))
             Sskip)
           (Ssequence
-            (Scall (Some 54%positive)
+            (Scall (Some 56%positive)
               (Evar _find_key (Tfunction
                                 (Tcons (tptr tint)
                                   (Tcons (tptr tint)
@@ -174,7 +176,7 @@ Definition f_find_key := {|
                (Etempvar _key tint) ::
                (Ebinop Osub (Etempvar _i tint) (Econst_int (Int.repr 1) tint)
                  tint) :: nil))
-            (Sreturn (Some (Etempvar 54%positive tint)))))))))
+            (Sreturn (Some (Etempvar 56%positive tint)))))))))
 |}.
 
 Definition f_get := {|
@@ -311,6 +313,67 @@ Definition f_erase := {|
               (Etempvar _index tint) (tptr tint)) tint)
           (Econst_int (Int.repr 0) tint))
         (Sreturn (Some (Econst_int (Int.repr 0) tint)))))))
+|}.
+
+Definition f_size_rec := {|
+  fn_return := tint;
+  fn_callconv := cc_default;
+  fn_params := ((_busybits, (tptr tint)) :: (_i, tint) :: nil);
+  fn_vars := nil;
+  fn_temps := ((_index, tint) :: (_bb, tint) :: (64%positive, tint) ::
+               (63%positive, tint) :: nil);
+  fn_body :=
+(Ssequence
+  (Sifthenelse (Ebinop Oeq (Econst_int (Int.repr 0) tint) (Etempvar _i tint)
+                 tint)
+    (Sreturn (Some (Econst_int (Int.repr 0) tint)))
+    Sskip)
+  (Ssequence
+    (Sset _index
+      (Ebinop Osub (Etempvar _i tint) (Econst_int (Int.repr 1) tint) tint))
+    (Ssequence
+      (Sset _bb
+        (Ederef
+          (Ebinop Oadd (Etempvar _busybits (tptr tint))
+            (Etempvar _index tint) (tptr tint)) tint))
+      (Ssequence
+        (Sifthenelse (Ebinop Oeq (Econst_int (Int.repr 1) tint)
+                       (Etempvar _bb tint) tint)
+          (Ssequence
+            (Scall (Some 63%positive)
+              (Evar _size_rec (Tfunction
+                                (Tcons (tptr tint) (Tcons tint Tnil)) tint
+                                cc_default))
+              ((Etempvar _busybits (tptr tint)) ::
+               (Ebinop Osub (Etempvar _i tint) (Econst_int (Int.repr 1) tint)
+                 tint) :: nil))
+            (Sreturn (Some (Ebinop Oadd (Econst_int (Int.repr 1) tint)
+                             (Etempvar 63%positive tint) tint))))
+          Sskip)
+        (Ssequence
+          (Scall (Some 64%positive)
+            (Evar _size_rec (Tfunction (Tcons (tptr tint) (Tcons tint Tnil))
+                              tint cc_default))
+            ((Etempvar _busybits (tptr tint)) ::
+             (Ebinop Osub (Etempvar _i tint) (Econst_int (Int.repr 1) tint)
+               tint) :: nil))
+          (Sreturn (Some (Etempvar 64%positive tint))))))))
+|}.
+
+Definition f_size := {|
+  fn_return := tint;
+  fn_callconv := cc_default;
+  fn_params := ((_busybits, (tptr tint)) :: nil);
+  fn_vars := nil;
+  fn_temps := ((65%positive, tint) :: nil);
+  fn_body :=
+(Ssequence
+  (Scall (Some 65%positive)
+    (Evar _size_rec (Tfunction (Tcons (tptr tint) (Tcons tint Tnil)) tint
+                      cc_default))
+    ((Etempvar _busybits (tptr tint)) :: (Econst_int (Int.repr 100) tint) ::
+     nil))
+  (Sreturn (Some (Etempvar 65%positive tint))))
 |}.
 
 Definition prog : Clight.program := {|
@@ -455,7 +518,9 @@ prog_defs :=
      tvoid cc_default)) :: (_loop, Gfun(Internal f_loop)) ::
  (_find_empty, Gfun(Internal f_find_empty)) ::
  (_find_key, Gfun(Internal f_find_key)) :: (_get, Gfun(Internal f_get)) ::
- (_put, Gfun(Internal f_put)) :: (_erase, Gfun(Internal f_erase)) :: nil);
+ (_put, Gfun(Internal f_put)) :: (_erase, Gfun(Internal f_erase)) ::
+ (_size_rec, Gfun(Internal f_size_rec)) :: (_size, Gfun(Internal f_size)) ::
+ nil);
 prog_main := _main
 |}.
 
